Finish atomic persist example

src/examples/atomic_persists.v
@@ -80,27 +80,55 @@ Section spec.
 
   Definition lock_res : dProp Σ :=
     ∃ ss b,
-      flush_lb x prot_bool b ∗
-      flush_lb y prot_bool b ∗
-      x ↦_{prot_bool} (ss ++ [b]) ∗
-      y ↦_{prot_bool} (ss ++ [b]).
+      "#pLbX" ∷ persist_lb x prot_bool false ∗
+      "#pLbY" ∷ persist_lb y prot_bool false ∗
+      "#fLbX" ∷ flush_lb x prot_bool b ∗
+      "#fLbY" ∷ flush_lb y prot_bool b ∗
+      "xPts" ∷ x ↦_{prot_bool} (ss ++ [b]) ∗
+      "yPts" ∷ y ↦_{prot_bool} (ss ++ [b]).
 
   Definition lock_condition : dProp Σ :=
     (* [x] and [y] *)
-    (∃ (xss yss : list bool) (bx byy : bool),
-      "#xPer" ∷ flush_lb x prot_bool bx ∗
-      "#yPer" ∷ flush_lb y prot_bool byy ∗
+    (∃ (xss yss : list bool) (bx byy : bool) bx' by',
+      "#pLbX" ∷ persist_lb x prot_bool bx' ∗
+      "#pLbY" ∷ persist_lb y prot_bool by' ∗
       "xPts" ∷ x ↦_{prot_bool} (xss ++ [bx]) ∗
       "yPts" ∷ y ↦_{prot_bool} (yss ++ [byy])).
 
+  Lemma lock_condition_impl bx' by' bx byy xss yss :
+    persist_lb x prot_bool bx' -∗
+    persist_lb y prot_bool by' -∗
+    x ↦_{prot_bool} (xss ++ [bx]) -∗
+    y ↦_{prot_bool} (yss ++ [byy]) -∗
+    <PC> lock_condition.
+  Proof.
+    iIntros "flX flY xPts yPts".
+    iCrashIntro.
+    iDestruct "flX" as "[pLbX (% & ? & xCrashed)]".
+    iDestruct "flY" as "[pLbY (% & ? & yCrashed)]".
+    iDestruct (crashed_in_if_rec with "xCrashed xPts")
+      as (??) "(? & crashedIn2 & xPts)".
+    iDestruct (crashed_in_if_rec with "yCrashed yPts")
+      as (??) "(? & crashedInY & yPts)".
+    repeat iExists _.
+    iFrameF "pLbX".
+    iFrameF "pLbY".
+    iFrame "xPts".
+    iFrame "yPts".
+  Qed.
+
+  Ltac solve_lc :=
+    try iModIntro (|={_}=> _)%I;
+    iDestruct (lock_condition_impl with "pLbX pLbY xPts yPts") as "$".
+
   Definition crash_condition : dProp Σ :=
-    (∃ (zss : list bool) (bz : bool),
-      "#zPer" ∷ persist_lb z prot_z bz ∗
+    (∃ (zss : list bool) (bz : bool) bz',
+      "#zPerLb" ∷ persist_lb z prot_z bz' ∗
       "zPts" ∷ z ↦_{prot_z} (zss ++ [bz])).
 
-  Lemma crash_condition_impl :
-    persist_lb z prot_z false -∗
-    z ↦_{prot_z} [false] -∗
+  Lemma crash_condition_impl_alt zss bz b :
+    persist_lb z prot_z b -∗
+    z ↦_{prot_z} (zss ++ [bz]) -∗
     <PC> crash_condition.
   Proof.
     iIntros "zPerLb zPts".
@@ -109,14 +137,24 @@ Section spec.
     iDestruct (crashed_in_if_rec with "crashedIn zPts")
       as (??) "(? & crashedIn2 & zPts)".
     simpl.
-    iExists _, _.
+    iExists _, _, _.
     iFrame "zPts".
     iApply (crashed_in_persist_lb with "crashedIn2").
   Qed.
 
+  Lemma crash_condition_impl bz b :
+    persist_lb z prot_z b -∗
+    z ↦_{prot_z} [bz] -∗
+    <PC> crash_condition.
+  Proof. iApply (crash_condition_impl_alt [] bz b). Qed.
+
   Ltac solve_cc :=
     try iModIntro (|={_}=> _)%I;
     iDestruct (crash_condition_impl with "zPerLb zPts") as "$".
+
+  Ltac solve_cc_alt :=
+    try iModIntro (|={_}=> _)%I;
+    iDestruct (crash_condition_impl_alt with "zPerLb zPts") as "$".
 
   Global Instance buffer_free_view_objective (P : dProp Σ) :
     ViewObjective P → BufferFree P.
@@ -165,134 +203,194 @@ Section spec.
       rewrite -2!persist_lb_to_flush_lb.
       iFrame "xPerLb yPerLb xPts yPts". }
     { iModIntro.
-      rewrite /lock_res /lock_condition.
-      iIntros "(% & % & xPts & yPts)".
-      iCrashIntro. admit. }
+      iNamed 1.
+      iApply (lock_condition_impl with "pLbX pLbY xPts yPts"). }
     iSplit; first solve_cc.
     iIntros (lk γ) "#isLock".
     wpc_pures; first solve_cc.
 
     wpc_bind (Fork _)%E.
     iApply (wpc_fork with "[]").
-    - (* Show safety of the forked off thread. *)
+    - (* Show safety of the forked off thread. I.e., the _left_ thread. *)
       iNext.
       wpc_apply (with_lock_spec with "[$isLock]"); first done.
       iSplit; first done.
-      (* iIntros "[borrow locked]". *)
-      (* wp_pures. *)
-      (* rewrite wp_wpc. *)
-      (* wpc_apply (use_crash_locked with "burrow"). *)
-      (* { done. } *)
-      (* iApply (wpc_crash_borrow_open with "borrow"). *)
-      (* { done. } *)
-      (* iSplit; first done. *)
-      iIntros "(% & % & ? & ? & xPts & yPts)".
+      setoid_rewrite (left_id (True%I) _ _).
+      iNamed 1.
       (* write to [x] *)
       wpc_bind (_ <-_NA _)%E.
       iApply wpc_atomic_no_mask.
       iSplit.
-      { admit. }
+      { solve_lc. }
       iApply (wp_store_na _ prot_bool _ _ b true with "[$xPts]"); eauto.
       { rewrite last_snoc. done. }
       { destruct b; done. }
       iNext. iIntros "xPts".
       iSplit.
-      { admit. }
+      { solve_lc. }
       iModIntro.
-      wpc_pures.
-      { admit. }
+      wpc_pures. { solve_lc. }
 
       (* write to [y] *)
       wpc_bind (_ <-_NA _)%E.
       iApply wpc_atomic_no_mask.
-      iSplit.
-      { admit. }
+      iSplit. { solve_lc. }
       iApply (wp_store_na _ prot_bool _ _ b true with "[$yPts]"); eauto.
       { rewrite last_snoc. done. }
       { destruct b; done. }
       iNext. iIntros "yPts".
-      iSplit. { admit. }
+      iSplit. { solve_lc. }
       iModIntro.
 
       (* flushes *)
-      wpc_pures.
-      { admit. }
+      wpc_pures. { solve_lc. }
 
       wpc_bind (Flush _)%E.
       iApply wpc_atomic_no_mask.
-      iSplit. { admit. }
+      iSplit. { solve_lc. }
       iApply (wp_flush_na with "xPts").
       iNext.
       iIntros "(xPts & #xLowerBound & ?)".
-      iSplit. { admit. }
+      iSplit. { solve_lc. }
       iModIntro.
 
       wpc_pures.
-      { admit. }
+      { solve_lc. }
 
       wpc_bind (Flush _)%E.
       iApply wpc_atomic_no_mask.
-      iSplit. { admit. }
+      iSplit. { solve_lc. }
       iApply (wp_flush_na with "yPts").
       iNext.
       iIntros "(yPts & #yLowerBound & ?)".
-      iSplit. { admit. }
+      iSplit. { solve_lc. }
       iModIntro.
 
       wpc_pures.
-      { admit. }
+      { solve_lc. }
 
-      iApply wpc_atomic_no_mask.
-      iSplit. { admit. }
+      iApply wpc_atomic_no_mask. iSplit. { solve_lc.  }
       wp_apply wp_fence.
       iModIntro. iModIntro.
       iSplit.
-      { admit. }
-      { admit. }
-    -
+      { solve_lc. }
+      iModIntro. rewrite left_id.
+      iExists _, true.
+      iFrameF "pLbX". iFrameF "pLbY". iFrameF "xLowerBound".
+      iFrameF "yLowerBound". iFrameF "xPts". iFrame "yPts".
+    - (* verify the _right_ thread. *)
       iSplit; first solve_cc.
       iNext.
       wpc_pure1 _; first solve_cc.
       wpc_pure1 _; first solve_cc.
       wpc_apply (with_lock_spec with "[$isLock zPts]"); first done.
       iSplit; first solve_cc.
-      iIntros "(% & % & #xLb & #yLb & xPts & yPts)".
+      iNamed 1.
 
       wpc_bind (!_NA _)%E.
       iApply wpc_atomic_no_mask.
       iSplit.
-      { solve_cc. admit. }
+      { solve_lc. solve_cc. }
       iApply (wp_load_na with "[$yPts]").
       { apply last_snoc. }
       { iModIntro.
         iIntros (?). iIntros "#H". iFrame "H". rewrite right_id. iApply "H". }
       iNext. iIntros (?) "[yPts ->]".
-      iSplit. { solve_cc. admit. }
+      iSplit. { solve_lc. solve_cc. }
       iModIntro.
       destruct b.
-      * wpc_pures. { solve_cc. admit. }
+      * wpc_pures. { solve_lc. solve_cc. }
         iApply wpc_atomic_no_mask.
-        iSplit. { solve_cc. admit. }
+        iSplit. { solve_lc. solve_cc. }
         iApply (wp_store_na _ prot_z _ _ _ true with "[$zPts]"); eauto.
         { simpl. iSplitPure; first done.
-          iFrame "xLb". done. }
+          iFrame "fLbX". done. }
         iNext. iIntros "zPts".
         iSplit.
-        { admit. }
-        { admit. }
-      * wpc_pures.
-        { solve_cc. admit. }
+        { solve_lc. solve_cc_alt. }
         iModIntro.
+        solve_cc_alt.
+        iExists _, true.
+        iFrameF "xPerLb". iFrameF "yPerLb". iFrameF "fLbX". iFrameF "fLbY".
+        iFrameF "xPts". iFrame "yPts".
+      * wpc_pures.
+        { solve_lc. solve_cc. }
+        iModIntro.
+        rewrite right_id.
         solve_cc.
-        admit.
-  Abort.
+        iExists _, false.
+        iFrameF "xPerLb". iFrameF "yPerLb". iFrameF "fLbX". iFrameF "fLbY".
+        iFrameF "xPts". iFrame "yPts".
+  Qed.
+
+  Instance if_else_persistent {PROP : bi} (b : bool) (P Q : PROP) :
+    Persistent P →
+    Persistent Q →
+    Persistent (if b then P else Q).
+  Proof. intros ??. destruct b; done. Qed.
 
   Lemma recovery_prog_spec s E :
-    crash_condition -∗
+    crash_condition ∗ lock_condition -∗
     WPC recovery x y z @ s; E
       {{ _, True }}
-      {{ <PC> crash_condition }}.
+      {{ (<PC> crash_condition) ∗ <PC> lock_condition }}.
   Proof.
-  Abort.
+    iIntros "[A B]".
+    iNamed "A".
+    iNamed "B".
+    rewrite /recovery.
+
+    (* load [z] *)
+    wpc_bind (!_NA _)%E.
+    iApply wpc_atomic_no_mask.
+    iSplit. { solve_cc_alt. solve_lc. }
+
+    iApply (wp_load_na with "[$zPts]").
+    { apply last_snoc. }
+    { iIntros "!>" (?) "#H". iFrame "H". rewrite right_id. iApply "H". }
+    iNext. iIntros (?) "[zPts #H]".
+    iSplit. { solve_cc_alt. solve_lc. }
+    iModIntro.
+    simpl.
+    destruct bz.
+    - iDestruct "H" as (->) "[flushX flushY]".
+      rewrite /assert.
+      wpc_pures. { solve_cc_alt. solve_lc. }
+
+      iDestruct (mapsto_na_store_lb_incl with "[] xPts") as %incl.
+      { iApply flush_lb_to_store_lb. iApply "flushX". }
+      inversion incl.
+      iDestruct (mapsto_na_store_lb_incl with "[] yPts") as %inclY.
+      { iApply flush_lb_to_store_lb. iApply "flushY". }
+      inversion inclY.
+
+      wpc_bind (!_NA _)%E.
+      iApply wpc_atomic_no_mask.
+      iSplit. { solve_lc. solve_cc_alt. }
+      iApply (wp_load_na with "[$xPts]").
+      { apply last_snoc. }
+      { iModIntro.
+        iIntros (?). iIntros "#H". iFrame "H". rewrite right_id. iApply "H". }
+      iNext. iIntros (?) "[xPts ->]".
+      iSplit. { solve_lc. solve_cc_alt. }
+      iModIntro.
+      wpc_pures. { solve_cc_alt. solve_lc. }
+
+      wpc_bind (!_NA _)%E.
+      iApply wpc_atomic_no_mask.
+      iSplit. { solve_lc. solve_cc_alt. }
+      iApply (wp_load_na with "[$yPts]").
+      { apply last_snoc. }
+      { iModIntro.
+        iIntros (?). iIntros "#H". iFrame "H". rewrite right_id. iApply "H". }
+      iNext. iIntros (?) "[yPts ->]".
+      iSplit. { solve_lc. solve_cc_alt. }
+      iModIntro.
+      wpc_pures. { solve_cc_alt. solve_lc. }
+      iModIntro. done.
+    - iDestruct "H" as %->.
+      wpc_pures. { solve_cc_alt. solve_lc. }
+      iModIntro. done.
+  Qed.
 
 End spec.
